Arithmetic/theories/Theorems.v
@@ -1,11 +1,154 @@
 From Coq Require Import ZArith.ZArith Strings.String.
 From RAC Require Import Utils Environnement Macros Oracle Translation.
-From RAC.Languages Require Import Syntax Semantics.
+From RAC.Languages Require Import Syntax Semantics MiniFSL.Semantics.
 
 Open Scope utils_scope.
 
 From RecordUpdate Require Import RecordUpdate.
 Import RecordSetNotations.
+Import FunctionalEnv FunctionalEnv.Domain.
+
+
+Fixpoint flatten {S T}  (s: @_c_statement S T) : list (@_c_statement S T) := match s with
+| Seq s1 s2 => flatten s1 ++ flatten s2
+| Skip => nil
+| _ => s::nil
+end
+.
+
+Definition unflatten {S T}  : list (@_c_statement S T) -> @_c_statement S T := fun l =>
+    List.fold_left (fun new_s  s => Seq new_s s) l Skip
+.
+
+Fact flatten_noseq_noskip {S T} s : List.Forall (fun i => i <> Skip /\ forall s1 s2, i <> @Seq S T s1 s2) (@flatten S T s).
+Admitted.
+
+Fact flatten_unflatten {S T} {ext_exp} {ext_stmt} {ext_stmt_vars} : forall f e e' s, 
+    @generic_stmt_sem S T ext_exp ext_stmt ext_stmt_vars f e s e' ->
+    @generic_stmt_sem S T ext_exp ext_stmt ext_stmt_vars f e (unflatten (flatten s)) e.
+Admitted.
+
+Lemma flatten_unique {S T} {ext_exp} {ext_stmt} {ext_stmt_vars} : forall s s' f e e', 
+    flatten s = flatten s' ->
+    @generic_stmt_sem S T ext_exp ext_stmt ext_stmt_vars f e s e' ->
+    @generic_stmt_sem S T ext_exp ext_stmt ext_stmt_vars f e s' e'.
+Proof.
+    assert (Hcon_nil_not : forall X (x :X) a b, x :: nil <> a ++ b). {
+        intros X x a b H. pose proof (List.nil_cons ). destruct b. simpl in H. admit. admit.
+    }
+    assert (Hnil: forall s f e, flatten s = nil <-> @generic_stmt_sem S T ext_exp ext_stmt ext_stmt_vars f e s e) by admit.
+    assert (Hsmth: forall s s' f e e',  
+                s :: nil = flatten s' -> 
+                @generic_stmt_sem S T ext_exp ext_stmt ext_stmt_vars f e s e' ->
+                @generic_stmt_sem S T ext_exp ext_stmt ext_stmt_vars f e s' e'
+        ) by admit.
+
+    intros s. induction s; intros  s' f  env env' Hflat Hsem ; simpl in Hflat.
+    - inversion Hsem.  destruct s'; subst; try discriminate.
+        + assumption.
+        + assert (flatten s'1 = nil /\ flatten s'2 = nil) as [Hs'1 Hs'2] by admit.
+            apply (Hnil _ f env') in Hs'2, Hs'1. now apply S_Seq with env'.
+    - now apply Hsmth with (f:=f) (e:=env)  (e':=env') in Hflat.
+    - now apply Hsmth with (f:=f) (e:=env)  (e':=env') in Hflat.
+    - now apply Hsmth with (f:=f) (e:=env)  (e':=env') in Hflat.
+    - subst. destruct (flatten s1) eqn:s1Eqn.
+        + simpl in Hflat.  specialize (IHs2 <{s'}> f env env'). apply IHs2 ; [assumption|]. clear IHs2. 
+            apply (Hnil _ f env) in s1Eqn. inversion Hsem; subst. admit.
+        + admit.
+Admitted.
+
+
+(* Compute (flatten  (Seq (Seq (Assign "x" 1) (Assign "x" 2)) (Assign "x" 3))).
+Compute (flatten  (Seq (Assign "x" 1) (Seq  (Assign "x" 2) (Assign "x" 3)))).
+Compute flatten ((Seq (Seq (Assign "x" 1) (Assign "x" 2)) (Seq (Assign "x" 3) (Assign "x" 4)))). *)
+
+
+
+(* [between left x right s] means [x] is between [left] and [right] inside [s] *)
+
+Inductive between : gmp_statement -> gmp_statement -> gmp_statement -> gmp_statement ->  Prop :=
+| Between_base : forall s1 s s2 s_whole, 
+    flatten s_whole = flatten s1 ++ flatten s ++ flatten s2 -> 
+    between s1 s s2 s_whole
+| Between_add_l s1 s_whole : forall s1' s s2 s_whole',
+    between s1 s s2 s_whole ->
+    flatten s_whole' = flatten s1'++ flatten s_whole ->
+    between s1' s s2 s_whole'
+
+| Between_add_r s2 s_whole : forall s1 s  s2' s_whole',
+    between s1 s s2 s_whole ->
+    flatten s_whole' = flatten s_whole ++ flatten s2' ->
+    between s1 s s2' s_whole' 
+.
+
+(* Goal forall s1 s2 s3 s4, between s1 s2 s4  (Seq (Seq s1 (Seq s2 s3)) s4).
+Proof.
+    intros. eapply (Between_add_r s3 (Seq s1 (Seq s2 s3))).
+    - now constructor.
+    - auto.
+Qed.
+
+Goal forall s1 s2 s3 s4, between s1 s2 s4  (Seq s1 (Seq s2 (Seq s3 s4))).
+Proof.
+    intros. eapply (Between_add_r s3 (Seq s1 (Seq s2 s3))).
+    - now constructor.
+    - simpl. now repeat rewrite <- List.app_assoc.
+Qed.
+
+Goal forall s1 s2 s3 s4, between s1 s3 s4  (Seq s1 (Seq s2 (Seq s3 s4))).
+Proof.
+    intros. eapply (Between_add_l s2 <{s2;s3;s4}>).
+    - now constructor. 
+    - simpl. now repeat rewrite <- List.app_assoc.
+Qed.
+
+
+Goal forall s1 s2 s3 s4, between s1 s2 s4  (Seq (Seq s1 s2) (Seq s3 s4)).
+    intros. eapply (Between_add_r s3 (Seq (Seq s1 s2) s3)).
+    - constructor. simpl. now rewrite <- List.app_assoc.
+    - simpl. now repeat rewrite <- List.app_assoc.  
+Qed. *)
+
+
+Definition In_stmt {S T} (s s' : @_c_statement S T) : Prop := List.In s (flatten s').
+
+
+Definition Forall_routines {F S T } (pgrm : @_c_program F S T) 
+    (PFuns : @_c_decl T * -> @_c_decl T * -> @_c_statement S T  -> Prop)
+    (* (PLFun : fsl_statement -> Prop)
+    (PPred : fsl_statement -> Prop) *)
+     : Prop :=
+    List.Forall (fun f => match f with
+        | PFun _ _ args decls body => PFuns args decls body
+        (* | F_Ext (LFun _ _ _ _) => True
+        | F_Ext (Predicate _ _ _) => True *)
+        | _ => True
+        end
+    ) (snd pgrm)
+.
+
+
+(* 
+    well_formed_program :
+    - all variables declared before usage
+    - all functions defined before called
+    - well typed
+*)
+Definition well_formed_pgrm (P : fsl_pgrm) (env : Env) (fenv: @fenv _fsl_statement Empty_set) := 
+    Forall_routines P ( fun args decls b =>
+        (* all used variables are declared *)
+        (forall v, List.In v (fsl_stmt_vars b) -> v ∈ env) /\ 
+        (* all functions are defined before being called *)
+        (forall rvar fname args, 
+            @In_stmt _fsl_statement Empty_set (FCall rvar fname args) b -> 
+            fname ∈ fenv.(funs)
+        
+        ) /\
+        True (* fixme: well typed ? *)
+    )
+.
+
+
 
 Module Theorems(Oracle:Oracle).
     
@@ -16,47 +159,95 @@ Module Theorems(Oracle:Oracle).
     (* -> Languages/{MiniC,MiniGMP}/Lemmas.v *)
 
 
-
-
     (* Section D : PROOFS OF STRUCTURAL PROPERTIES OF THE TRANSLATION *)
 
-    Lemma LD1_mpz_pointer_invariant : forall P args env env',
-        (gmp_pgrm_sem env (T.translate_program P) args env')  -> True.
+
+    (* `if the generated program has a semantic [...]'  but no semantic given for a program   *)
+    Lemma LD1_mpz_pointer_invariant : forall P fenv t_fenv env,
+        well_formed_pgrm  P env fenv ->
+        Forall_routines (T.translate_program P) ( fun _ _ b => 
+            forall (renv renv' : Env),
+            forall v, type_of_value (renv v) = Some (T_Ext Mpz) ->
+            forall s, between <( init(v) )> s <( cl(v) )> b -> 
+            (renv |= s => renv')%gmpssem t_fenv ->
+            renv v = renv' v
+        )
+    .
     Proof.
-    auto.
-    Qed.
+        intros P args env env' Hwf. unfold Forall_routines. apply List.Forall_forall. intros R Hr. destruct R eqn:REqn;[|trivial].
+        intros renv renv' v Hv stmt Hstmt Hsem. 
+        (* unroll translation... *)
+        destruct P as [Pdecls Pfuns]. destruct Pfuns eqn:PfunsEqn; simpl in Hr; [easy|]. 
+        destruct Pdecls eqn:PdeclsEqn; simpl in Hr. admit.
+    Admitted.
 
-    Lemma LD2_absence_of_aliasing : True.
+    Lemma LD2_absence_of_aliasing : forall P fenv t_fenv env,
+        well_formed_pgrm  P env fenv ->
+        Forall_routines (T.translate_program P) ( fun _ _ b => 
+            forall s (renv renv' : Env),
+            (renv |= s => renv')%gmpssem t_fenv ->
+            forall v (l:location), renv' v = Some (Def (VMpz l)) ->
+            forall v' (l':location), v' <> v /\ renv' v' =  Some (Def (VMpz l')) ->
+            l <> l'
+        )
+    .
     Proof.
-        auto.
-    Qed.
+        intros P args env env' Hwf. unfold Forall_routines. apply List.Forall_forall. intros R Hr. destruct R eqn:REqn;[|trivial].
+        intros renv renv' v Hv stmt Hstmt Hsem. 
+        (* unroll translation... *)
+        destruct P as [Pdecls Pfuns]. destruct Pfuns eqn:PfunsEqn; simpl in Hr; [easy|]. 
+        destruct Pdecls eqn:PdeclsEqn; simpl in Hr. admit.
+    Admitted.
 
-    Lemma LD3_preservation_of_control_flow : True.
+
+    Lemma LD3_preservation_of_control_flow : forall P fenv env,
+        well_formed_pgrm  P env fenv ->
+        Forall_routines (T.translate_program P) ( fun _ _ b => 
+            forall decls s,
+            In_stmt (S_Ext (GMP_Scope decls s)) b -> 
+            (* passes through: how to represent control flow ?  *)
+            True
+        )
+    .
+    Admitted.
+
+    Lemma LD4 : forall P env fenv,
+        well_formed_pgrm  P env fenv ->
+        (* translate_predicate ... *)
+        True.
     Proof.
-        auto.
-    Qed.
+    Admitted.
 
-    Lemma LD4 : True.
+
+    Lemma LD5_memory_transparency_of_generated_code : forall P fenv env,
+        well_formed_pgrm  P env fenv ->
+        Forall_routines (T.translate_program P) ( fun _ _ b => 
+            forall decls s,
+            In_stmt (S_Ext (GMP_Scope decls s)) b -> 
+            (* todo: add decls tec *)
+            True
+        )
+    .
     Proof.
-        auto.
-    Qed.
+    Admitted.
 
-
-    Lemma LD5_memory_transparency_of_generated_code : True.
-    Proof.
-        auto.
-    Qed.
-
-    Theorem T61_absence_of_dangling_pointers : True. 
+    Theorem T61_absence_of_dangling_pointers : forall P fenv t_fenv env,
+        well_formed_pgrm  P env fenv ->
+        Forall_routines (T.translate_program P) ( fun _ _ b => 
+            forall s (renv renv' : Env),
+            (renv |= s => renv')%gmpssem t_fenv ->
+            forall (l:location), renv'.(mstate) l <> None <->  exists! x, eq (renv' x) (Some (Def (VMpz l)))
+        ). 
     Proof. 
-        auto.
-    Qed.
+    Admitted.   
 
-
-    Theorem T62_absence_of_memory_leak : True. 
+    Theorem T62_absence_of_memory_leak :  forall P args fenv env env',
+        well_formed_pgrm  P env fenv ->
+        gmp_pgrm_sem env (T.translate_program P) args env' ->
+        env'.(mstate) = ⊥
+    .
     Proof. 
-        auto.
-    Qed.
+    Admitted.
 
 
     (* Section E : PROOFS OF THE SEMANTICS OF THE MACROS *)
@@ -87,13 +278,6 @@ Inductive pgrm_var_representation (iop:ϴ) (e : Env) (ienv:Γ) : Env -> Prop :=
     add_var_𝐴 e A {|env:=ΩΓ; mstate:=𝓜Γ|} -> 
     pgrm_var_representation iop e ienv{|env:=ΩΓ; mstate:=𝓜Γ|}
 .
-
-(* Definition well_formed_program :=
-    - all variables declared before usage
-    - all functions defined before called
-    - well typed
-*)
-
 
 *)
 
